merge impl.v

cryptis/sess/impl.v
@@ -6,27 +6,30 @@ From iris.algebra Require Import max_prefix_list.
 From iris.heap_lang Require Import notation proofmode.
 From cryptis Require Import lib term cryptis primitives tactics.
 From cryptis Require Import role iso_dh conn.
-From actris Require Import proto.
+From cryptis.examples Require Import iso_dh gen_conn.
+From actris.channel Require Import proto.
 
+From cryptis.examples.gen_conn.proofs Require Import base.
 
 Set Implicit Arguments.
 Unset Strict Implicit.
 Unset Printing Implicit Defensive.
 
 Notation sessN := (nroot.@"sess").
+Local Notation connN := (nroot.@"conn").
 
 Module Impl.
 
 Section Impl.
 
 Definition connect : val := λ: "c" "skA" "pkB",
-  let: "conn" := Conn.connect "c" "skA" "pkB" in
+  let: "conn" := GenConn.connect "c" "skA" "pkB" in
   (#true, "conn").
 
-Definition listen : val := λ: "c", Conn.listen "c".
+Definition listen : val := λ: "c", GenConn.listen "c".
 
 Definition confirm : val := λ: "c" "skB" "req",
-  let: "conn" := Conn.confirm "c" "skB" "req" in
+  let: "conn" := GenConn.confirm "c" "skB" "req" in
   (#false, "conn").
 
 Definition send : val := λ: "cs" "ts",
@@ -34,15 +37,253 @@ Definition send : val := λ: "cs" "ts",
   let: "conn" := Snd "cs" in
   let: "N" := if: "is_init" then Tag (sessN.@"init") else
               Tag (sessN.@"resp") in
-  Conn.send "conn" "N" "ts".
+  GenConn.send "conn" "N" "ts".
 
 Definition recv : val := λ: "cs",
   let: "is_init" := Fst "cs" in
   let: "conn" := Snd "cs" in
   let: "N" := if: "is_init" then Tag (sessN.@"resp") else
               Tag (sessN.@"init") in
-  Conn.recv "conn" "N".
+  GenConn.recv "conn" "N".
 
 End Impl.
 
 End Impl.
+
+Section Proofs.
+  Notation iProto Σ := (iProto Σ term).
+  Notation iMsg Σ := (iMsg Σ term).
+
+  Record params Σ := Params {
+  chan_inv :
+    sign_key → sign_key → sess_info → list term → list term → iProp Σ;
+  msg_inv :
+    sign_key → sign_key → sess_info → role → term → iProp Σ;
+                       }.
+
+  Context `{!cryptisGS Σ, !heapGS Σ, !GenConn.connGS Σ, !protoG Σ term}.
+  Notation iProp := (iProp Σ).
+
+  Implicit Types (cs : GenConn.state).
+  Implicit Types (kS t : term) (ts : list term).
+  Implicit Types (skI skR : sign_key).
+  Implicit Types n m : nat.
+  Implicit Types b : bool.
+  Implicit Types v : val.
+  Implicit Types (ok : Prop) (failed : bool).
+  Implicit Types (si : sess_info) (rl : role).
+  (* Implicit Types (ps : params Σ). *)
+  Implicit Types (p : iProto Σ).
+  Implicit Types (N : namespace).
+
+  (* Variable term_to_val : term → val. *)
+  (* Variable val_to_term : val → term. *)
+  Search term_meta.
+
+
+Definition proto_msg_pred skI skR si rl t : iProp :=
+  True.
+
+Definition proto_chan_pred skI skR si rl t : iProp :=
+  True.
+
+  Definition iProto_pointsto
+    N (rl : role) cs (p : iProto Σ) : iProp :=
+    ∃ γ
+      (* γr *)
+      ,
+        (* skI γl *)
+        (if rl is Init then
+          term_meta (si_init_share cs) N γ
+          else term_meta (si_resp_share cs) N γ )
+                         ∗
+        (* term_meta γl N  *)
+      (* chan_inv () ∗ *)
+    iProto_own γ p.
+
+
+Definition prot_connected N p ps skI skR rl cs : iProp :=
+  connected ps skI skR rl cs ∗
+            iProto_pointsto N rl cs p.
+            (* ∗ *)
+    (* ∃ γ, iProto_own γ prot. *)
+
+Definition my_msg_inv `{!heapGS Σ}
+    (p : iProto Σ) (skI skR : sign_key) (cs : sess_info) (rl : role) (t :term) : iProp  :=
+    ∃ (p' : iProto Σ) (P : iProp Σ),
+      (* let v := term_to_val t in *)
+       iMsg_car (MSG (term_to_val t) {{P}}; p') \/ (Next p').
+
+
+            Lemma wp_connect P p c skI skR :
+  channel c -∗
+  cryptis_ctx -∗
+  ctx -∗
+  minted skI -∗
+  minted skR -∗
+  {{{ GenConn.failure skI skR ∨ P }}}
+    impl.connect c skI (Spec.pkey skR)
+  {{{ cs, RET (repr cs);
+      prot_connected N p skI skR Init cs ∗
+      (compromised cs ∨ P) }}}.
+
+
+Definition connected skI skR rl cs : iProp :=
+  GenConn.connected {| GenConn.chan_inv := proto_chan_pred; GenConn.msg_inv := proto_chan_pred |}
+    skI skR rl cs.
+
+Definition proto_tokens cs : iProp :=
+  True.
+  (* public (si_key cs) ∨ *)
+  (* resp_pred_token cs rpcN (TInt 0) ∗ *)
+  (* resp_pred_token cs rpcN (TInt 0). *)
+
+
+Definition proto_connected kI kR cs : iProp :=
+  connected kI kR Init cs ∗
+  release_token (si_init_share cs) ∗
+  proto_tokens cs.
+
+Lemma wp_connect P c skI skR :
+  channel c -∗
+  cryptis_ctx -∗
+  ctx -∗
+  minted skI -∗
+  minted skR -∗
+  {{{ GenConn.failure skI skR ∨ P }}}
+    impl.connect c skI (Spec.pkey skR)
+  {{{ cs, RET (repr cs);
+      proto_connected skI skR cs ∗
+      (compromised cs ∨ P) }}}.
+
+
+Lemma wp_connect P c skI skR N ps :
+  ctx N ps -∗
+  {{{(failure skI skR ∨ P)}}}
+    impl.connect c skI (Spec.pkey skR) (Tag N)
+    {{{cs, RET (repr cs); True}}}.
+
+Lemma my_wp_connect P c skI skR N ps :
+  channel c ∗
+  cryptis_ctx ∗
+  ctx N ps ∗
+  minted skI ∗
+  minted skR -∗
+  {{{ GenConn.failure skI skR ∨ P }}}
+    impl.connect c skI (Spec.pkey skR) (Tag N)
+  {{{ cs, RET (repr cs);
+      connected ps skI skR Init cs ∗
+      (public (si_key cs) ∨ P) ∗
+      release_token (si_init_share cs) ∗
+      term_token (si_init_share cs) (⊤ ∖ ↑iso_dhN ∖ ↑connN) }}}.
+Proof. exact: GenConn.wp_connect. Qed.
+
+(* Definition prot_pred N φ : iProp := *)
+(*   True%I. *)
+  (* nown iso_dh_name N *)
+  (*   (saved_pred DfracDiscarded (λ '(skI, skR, si, rl), φ skI skR si rl)). *)
+  Definition my_chan_inv `{!heapGS Σ, !protoG Σ term}
+     N (skI skR : sign_key) (cs : sess_info) (tsI tsR : list term) : iProp :=
+    ∃ ( yl yr : gname) , term_meta (si_init_share cs) N yl ∗ term_meta (si_resp_share cs) N yr ∗
+                           iProto_ctx yl yr tsI tsR.
+
+  Definition iProto_pointsto `{!heapGS Σ, !protoG Σ val}
+    N (rl : role) cs (p : iProto Σ) : iProp :=
+    ∃ γ
+      (* γr *)
+      ,
+        (* skI γl *)
+        (if rl is Init then
+          term_meta (si_init_share cs) N γ
+          else term_meta (si_resp_share cs) N γ )
+                         ∗
+        (* term_meta γl N  *)
+      (* chan_inv () ∗ *)
+    iProto_own γl p.
+
+
+Definition prot_connected prot ps skI skR rl cs : iProp :=
+  connected ps skI skR rl cs ∗
+            iProto_pointsto (* rl *) prot
+    ∃ γ, iProto_own γ prot.
+
+Lemma wp_initiator P :
+  Lemma wp_connect P prot_connected :
+
+Lemma wp_initiator failed c skI skR N φ :
+  channel c -∗
+  cryptis_ctx -∗
+  iso_dh_ctx -∗
+  iso_dh_pred N φ -∗
+  minted skI -∗
+  minted skR -∗
+  (if failed then public skI ∨ public skR else True) -∗
+  {{{ True }}}
+    initiator c skI (Spec.pkey skR) (Tag N)
+  {{{ okS, RET (repr okS);
+      if okS is Some kS then ∃ si,
+        ⌜si_init si = skI⌝ ∗
+        ⌜si_resp si = skR⌝ ∗
+        ⌜si_key si = kS⌝ ∗
+        minted kS ∗
+        session si ∗
+        □ (⌜failed⌝ → public (si_key si)) ∗
+        release_token (si_init_share si) ∗
+        term_token (si_init_share si) (⊤ ∖ ↑iso_dhN) ∗
+        (public (si_key si) ∨ φ skI skR si Init)
+      else True
+ }}}.
+
+Lemma wp_connect P c skI skR N ps :
+  channel c ∗
+  cryptis_ctx ∗
+  ctx N ps ∗
+  minted skI ∗
+  minted skR -∗
+  {{{ (failure skI skR ∨ P) }}}
+    impl.connect c skI (Spec.pkey skR) (Tag N)
+  {{{ cs, RET (repr cs);
+      connected ps skI skR Init cs ∗
+      (public (si_key cs) ∨ P) ∗
+      release_token (si_init_share cs) ∗
+      term_token (si_init_share cs) (⊤ ∖ ↑iso_dhN ∖ ↑connN) }}}.
+
+  Definition my_chan_inv `{!heapGS Σ, !protoG Σ term}
+     (skI skR : sign_key) (cs : sess_info) (tsI tsR : list term) : iProp :=
+    (* let vsI := List.map term_to_val tsI in *)
+    (* let vsR := List.map term_to_val tsR in *)
+
+    ∃ ( yl yr : gname) , term_meta cs N yl ∗ term_meta cs N yr ∗
+                           iProto_ctx yl yr tsI tsR.
+
+  Definition iProto_pointsto `{!heapGS Σ, !protoG Σ val}
+     (skI : sign_key) (p : iProto Σ) : iProp Σ :=
+    iProto_own skI p.
+  (* ∗ iProto_own yl pl ∗ iProto_own yr pr. *).
+
+  Print iMsg_base.
+
+  Definition my_msg_inv `{!heapGS Σ}
+    (p : iProto Σ) (skI skR : sign_key) (cs : sess_info) (rl : role) (t :term) : iProp  :=
+    ∃ (p' : iProto Σ) (P : iProp Σ),
+      (* let v := term_to_val t in *)
+       iMsg_car (MSG (term_to_val t) {{P}}; p') \/ (Next p').
+
+(* Definition my_params {Σ} `{!heapGS Σ, !chanG Σ} (p : iProto Σ) : params Σ := *)
+(*   Params (my_chan_inv p) (my_msg_inv p). *)
+
+  Definition my_gen_params p : GenConn.params Σ := {|
+    GenConn.chan_inv := my_chan_inv;
+    GenConn.msg_inv := my_msg_inv p;
+                                                  |}%I.
+
+
+  Definition wp_initiator
+
+  Definition iProto_pointsto_def `{!heapGS Σ}
+    (cs : val) (p : iProto Σ) : iProp Σ :=
+    ∃ cnts sess ch n,
+      ∗
+
+
+End Proofs.
